theories/Logic/MuRec.v
@@ -1,0 +1,473 @@
+Require Import PnV.Prelude.Prelude.
+Require Import PnV.Prelude.ConstructiveFacts.
+Require Import PnV.Data.Vector.
+Require Import PnV.Logic.PrimRec.
+
+Section UNBOUNDED_MINIMIZATION. (* Reference: "https://github.com/DmxLarchey/Murec_Extraction/blob/murec_artifact/theories/standalone.v" *)
+
+#[local] Infix "\in" := E.In : type_scope.
+#[local] Infix "\subseteq" := E.subset : type_scope.
+
+Section BETWEEN. (* Reference: "https://github.com/DmxLarchey/Murec_Extraction/blob/murec_artifact/theories/between.v" *)
+
+Variable P : nat -> Prop.
+
+Definition wBetween (n : nat) (m : nat) : Prop :=
+  forall i, n <= i -> i < m -> P i.
+
+Lemma wBetween_refl (n : nat)
+  : wBetween n n.
+Proof.
+  red. lia.
+Qed.
+
+Lemma wBetween_next (n : nat)
+  : forall m, wBetween n m -> P m -> wBetween n (S m).
+Proof.
+  ii. inv H2.
+  - trivial.
+  - eapply H; lia.
+Qed.
+
+Definition Between (n : nat) (m : nat) : Prop :=
+  n <= m /\ wBetween n m.
+
+Lemma Between_refl (n : nat)
+  : Between n n.
+Proof.
+  split. lia. eapply wBetween_refl.
+Qed.
+
+Lemma Between_next (n : nat)
+  : forall m, Between n m -> P m -> Between n (S m).
+Proof.
+  ii. destruct H. split.
+  - lia.
+  - eapply wBetween_next; trivial.
+Qed.
+
+End BETWEEN.
+
+Lemma Between_ind (P : nat -> Prop) (a : nat) (b : nat)
+  (H_Between : Between (fun n => P (S n) -> P n) a b)
+  : P b -> P a.
+Proof.
+  destruct H_Between as [a_le_b H_wBetween]. red in H_wBetween.
+  revert H_wBetween. induction a_le_b as [ | m LE IH].
+  - i. exact H.
+  - i. eapply IH.
+    + i. eapply H_wBetween.
+      * exact H0.
+      * exact (le_S (S i) m H1).
+      * exact H2.
+    + eapply H_wBetween.
+      * exact LE.
+      * exact (le_n (S m)).
+      * exact H.
+Defined.
+
+Variable F : nat -> nat -> Prop.
+
+Definition umin s y := F y 0 /\ Between (fun n => exists k, F n (S k)) s y.
+
+Definition umin' y :=  F y 0 /\ forall n, n < y -> exists k, F n (S k).
+
+Variable Ffun : forall x, forall y1, forall y2, F x y1 -> F x y2 -> y1 = y2.
+
+Variable f : forall x : nat, (exists y, F x y) -> { y : nat | F x y }.
+
+Let T n := exists k, F n k.
+
+Let P n := F n 0.
+
+Let Q n := exists k, F n (S k).
+
+Lemma PQ_absurd (n : nat)
+  : P n -> Q n -> False.
+Proof.
+  intros p (y & q). red in p. pose proof (Ffun n 0 (S y) p q) as H_false. inv H_false.
+Qed.
+
+Inductive Dumin (n : nat) : Prop :=
+  | Dumin_stop : T n -> P n -> Dumin n
+  | Dumin_next : T n -> Dumin (S n) -> Dumin n.
+
+#[local] Arguments Dumin_stop {_}.
+#[local] Arguments Dumin_next {_}.
+
+Definition Dumin_pi1 {n} (d : Dumin n) : T n :=
+  match d with
+  | Dumin_stop t _ => t
+  | Dumin_next t _ => t
+  end.
+
+Definition Dumin_pi2 {n} (d : Dumin n) : Q n -> Dumin (S n) :=
+  match d with
+  | Dumin_stop t p  => fun q => False_ind _ (PQ_absurd n p q)
+  | Dumin_next _ d' => fun _ => d'
+  end.
+
+Definition Pre_umin (s : nat) (n : nat) : Prop :=
+  n \in E.intersection (E.intersection T P) (Between T s).
+
+Definition Post_umin (s : nat) (n : nat) : Prop :=
+  n \in E.intersection (E.intersection T P) (Between (E.intersection T Q) s).
+
+Lemma Pre_umin_Dumin {s : nat}
+  (EXISTENCE : exists n, Pre_umin s n)
+  : Dumin s.
+Proof.
+  revert EXISTENCE. intros [n IN]. red in IN. s!. destruct IN as [[IN IN1] IN0].
+  pose proof (Dumin_stop IN IN1). revert H. eapply Between_ind.
+  do 2 red in IN0. des. red. split. exact IN0. ii. eapply Dumin_next; trivial. eapply IN2; trivial.
+Qed.
+
+Fixpoint loop (s : nat) (n : nat) (d : Dumin n) (b : Between Q s n) {struct d} : { x : nat | umin s x }.
+Proof.
+  pose proof (f n (Dumin_pi1 d)) as [k H_k]. revert H_k. destruct k as [ | k']; i.
+  - exists n. split.
+    + exact H_k.
+    + exact b.
+  - eapply loop with (n := S n).
+    + eapply Dumin_pi2.
+      * exact d.
+      * red. exists k'. exact H_k.
+    + eapply Between_next.
+      * exact b.
+      * red. exists k'. exact H_k.
+Defined.
+
+Let linear_search (s : nat) : (exists x, Pre_umin s x) -> { x : nat | umin s x } :=
+  fun EXISTENCE => loop s s (Pre_umin_Dumin EXISTENCE) (Between_refl Q s).
+
+Lemma umin_incl_Pre_umin (s : nat)
+  : umin s \subseteq Pre_umin s.
+Proof.
+  intros n IN. red. red. do 2 red in IN. destruct IN as [F_n_0 H_Between]. s!. split. split.
+  - red. red. exists 0. exact F_n_0.
+  - red. red. exact F_n_0.
+  - destruct H_Between as [LE H_wBetween]. split; trivial. ii. red.
+    pose proof (H_wBetween i H H0) as [k H_k]. exists (S k). exact H_k.
+Qed.
+
+Definition compute_umin (s : nat)
+  (EXISTENCE : exists x, umin s x)
+  : { x : nat | umin s x }.
+Proof.
+  eapply linear_search. destruct EXISTENCE as [x H_x]. exists x. eapply umin_incl_Pre_umin. exact H_x.
+Defined.
+
+Lemma compute_umin'
+  (EXISTENCE : exists x, umin' x)
+  : { x : nat | umin' x }.
+Proof.
+  assert (claim1 : exists x : nat, umin 0 x).
+  { destruct EXISTENCE as [x H_x]. exists x. red. red in H_x. destruct H_x as [H_x H_wBetween].
+    split; trivial. split. lia. ii. eapply H_wBetween. exact H0.
+  }
+  apply compute_umin with (s := 0) in claim1. destruct claim1 as [x H_x].
+  exists x. red. red in H_x. destruct H_x as [H_x H_Between]. split; trivial.
+  ii. destruct H_Between as [_ H_wBetween]. red in H_wBetween. eapply H_wBetween; lia.
+Qed.
+
+End UNBOUNDED_MINIMIZATION.
+
+Section MU_RECURSIVE.
+
+#[local] Close Scope list_scope.
+#[local] Open Scope vector_scope.
+
+#[local] Notation " [ ] " := (VNil).
+#[local] Notation " x :: xs " := (VCons _ x xs).
+#[local] Notation " [ x ] " := (VCons _ x VNil).
+
+Let Arity : Set := nat.
+
+Inductive MuRec : Arity -> Set :=
+  | MR_succ : MuRec 1
+  | MR_zero : MuRec 0
+  | MR_proj {n : Arity} (i : Fin.t n) : MuRec n
+  | MR_compose {n : Arity} {m : Arity} (g : MuRecs n m) (h : MuRec m) : MuRec n
+  | MR_primRec {n : Arity} (g : MuRec n) (h : MuRec (S (S n))) : MuRec (S n)
+  | MR_mu {n : Arity} (g : MuRec (S n)) : MuRec n
+with MuRecs : Arity -> Arity -> Set :=
+  | MRs_nil {n : Arity} : MuRecs n 0
+  | MRs_cons {n : Arity} {m : Arity} (f : MuRec n) (fs : MuRecs n m) : MuRecs n (S m).
+
+Let Value := nat.
+
+Inductive MuRecSpec : forall n : Arity, MuRec n -> Vector.t Value n -> Value -> Prop :=
+  | MR_succ_spec x
+    : MuRecSpec 1 (MR_succ) [x] (S x)
+  | MR_zero_spec
+    : MuRecSpec 0 (MR_zero) [] (O)
+  | MR_proj_spec n xs i
+    : MuRecSpec n (MR_proj i) xs (xs !! i)
+  | MR_compose_spec n m g h xs ys z
+    (g_spec : MuRecsSpec n m g xs ys)
+    (h_spec : MuRecSpec m h ys z)
+    : MuRecSpec n (MR_compose g h) xs z
+  | MR_primRec_spec_O n g h xs z
+    (g_spec : MuRecSpec n g xs z)
+    : MuRecSpec (S n) (MR_primRec g h) (O :: xs) z
+  | MR_primRec_spec_S n g h xs z a acc
+    (ACC : MuRecSpec (S n) (MR_primRec g h) (a :: xs) acc)
+    (h_spec : MuRecSpec (S (S n)) h (a :: acc :: xs) z)
+    : MuRecSpec (S n) (MR_primRec g h) (S a :: xs) z (* corrected by "SoonWon Moon" *)
+  | MR_mu_spec n g xs z
+    (g_spec : MuRecSpec (S n) g (z :: xs) 0)
+    (MIN : forall y, y < z -> exists p, p > 0 /\ MuRecSpec (S n) g (y :: xs) p) (* corrected by "SoonWon Moon" *)
+    : MuRecSpec n (MR_mu g) xs z
+with MuRecsSpec : forall n : Arity, forall m : Arity, MuRecs n m -> Vector.t Value n -> Vector.t Value m -> Prop :=
+  | MRs_nil_spec n xs
+    : MuRecsSpec n (O) (MRs_nil) xs []
+  | MRs_cons_spec n m xs y ys f fs
+    (f_spec : MuRecSpec n f xs y)
+    (fs_spec : MuRecsSpec n m fs xs ys)
+    : MuRecsSpec n (S m) (MRs_cons f fs) xs (y :: ys).
+
+Fixpoint MuRecGraph {n : Arity} (f : MuRec n) : Vector.t Value n -> Value -> Prop :=
+  match f with
+  | MR_succ => fun xs => fun z => S (V.head xs) = z
+  | MR_zero => fun xs => fun z => O = z
+  | MR_proj i => fun xs => fun z => xs !! i = z
+  | MR_compose g h => fun xs => fun z => exists ys, MuRecsGraph g xs ys /\ MuRecGraph h ys z
+  | MR_primRec g h => fun xs => nat_rect _ (fun z => MuRecGraph g (V.tail xs) z) (fun a => fun ACC => fun z => exists y, ACC y /\ MuRecGraph h (a :: y :: V.tail xs) z) (V.head xs)
+  | MR_mu g => fun xs => fun z => (forall y, y < z -> exists p, p > 0 /\ MuRecGraph g (y :: xs) p) /\ MuRecGraph g (z :: xs) 0 (* corrected by "SoonWon Moon" *)
+  end
+with MuRecsGraph {n : Arity} {m : Arity} (fs : MuRecs n m) : Vector.t Value n -> Vector.t Value m -> Prop :=
+  match fs with
+  | MRs_nil => fun xs => fun z => [] = z
+  | MRs_cons f fs => fun xs => fun z => exists y, exists ys, MuRecGraph f xs y /\ MuRecsGraph fs xs ys /\ y :: ys = z
+  end.
+
+Fixpoint MuRecGraph_sound (n : Arity) (f : MuRec n) {struct f}
+  : forall xs, forall z, MuRecGraph f xs z -> MuRecSpec n f xs z
+with MuRecsGraph_sound (n : Arity) (m : Arity) (fs : MuRecs n m) {struct fs}
+  : forall xs, forall z, MuRecsGraph fs xs z -> MuRecsSpec n m fs xs z.
+Proof.
+  - destruct f; intros xs z CALL.
+    + r in CALL. subst z. revert xs. introVCons x xs. revert xs. introVNil. cbv. econs 1.
+    + r in CALL. subst z. revert xs. introVNil. econs 2.
+    + r in CALL. subst z. econs 3.
+    + simpl in CALL. destruct CALL as (ys&CALLs&CALL). econs 4.
+      * eapply MuRecsGraph_sound. exact CALLs.
+      * eapply MuRecGraph_sound. exact CALL.
+    + simpl in CALL. revert xs CALL. introVCons a xs. revert z xs. induction a as [ | a ACC]; i.
+      * simpl in CALL. unfold V.tail in CALL. simpl in CALL. econs 5.
+        eapply MuRecGraph_sound. exact CALL.
+      * simpl in CALL. destruct CALL as [y [CALL IH]]. unfold V.tail in CALL. simpl in CALL. unfold V.tail in IH. simpl in IH. econs 6.
+        { eapply ACC with (z := y). exact CALL. }
+        { eapply MuRecGraph_sound. exact IH. }
+    + simpl in CALL. destruct CALL as [g_spec MIN]. econs 7.
+      * eapply MuRecGraph_sound. exact MIN.
+      * intros y y_lt_z. pose proof (g_spec y y_lt_z) as [p [p_gt_0 CALL]]. exists p. split. exact p_gt_0. eapply MuRecGraph_sound. exact CALL.
+  - destruct fs; intros xs z CALL.
+    + simpl in CALL. subst z. econs 1.
+    + simpl in CALL. destruct CALL as [y [ys [CALL [CALLs ?]]]]. subst z. econs 2.
+      * eapply MuRecGraph_sound. exact CALL.
+      * eapply MuRecsGraph_sound. exact CALLs.
+Qed.
+
+Fixpoint MuRecGraph_complete (n : Arity) (f : MuRec n) (xs : Vector.t Value n) (z : Value) (SPEC : MuRecSpec n f xs z) {struct SPEC}
+  : MuRecGraph f xs z
+with MuRecsGraph_complete (n : Arity) (m : Arity) (fs : MuRecs n m) (xs : Vector.t Value n) (z : Vector.t Value m) (SPEC : MuRecsSpec n m fs xs z) {struct SPEC}
+  : MuRecsGraph fs xs z.
+Proof.
+  - destruct SPEC; simpl.
+    + reflexivity.
+    + reflexivity.
+    + reflexivity.
+    + exists ys. split.
+      * eapply MuRecsGraph_complete. exact g_spec.
+      * eapply MuRecGraph_complete. exact SPEC.
+    + eapply MuRecGraph_complete. exact SPEC.
+    + exists acc. unfold V.tail. simpl. split.
+      * apply MuRecGraph_complete in SPEC1. exact SPEC1.
+      * apply MuRecGraph_complete in SPEC2. exact SPEC2.
+    + split.
+      * intros y y_lt_z. pose proof (MIN y y_lt_z) as [p [p_gt_0 SPEC']].
+        exists p. split. exact p_gt_0. eapply MuRecGraph_complete. exact SPEC'.
+      * eapply MuRecGraph_complete. exact SPEC.
+  - destruct SPEC; simpl.
+    + reflexivity.
+    + exists y, ys. split. 
+      * eapply MuRecGraph_complete. exact f_spec.
+      * split.
+        { eapply MuRecsGraph_complete. exact SPEC. }
+        { reflexivity. }
+Qed.
+
+Theorem MuRecGraph_correct (n : Arity) (f : MuRec n) (xs : Vector.t Value n) (z : Value)
+  : MuRecGraph f xs z <-> MuRecSpec n f xs z.
+Proof.
+  pose proof (LEFT := @MuRecGraph_complete). pose proof (RIGHT := @MuRecGraph_sound). now firstorder.
+Qed.
+
+Theorem MuRecsGraph_correct (n : Arity) (m : Arity) (f : MuRecs n m) (xs : Vector.t Value n) (z : Vector.t Value m)
+  : MuRecsGraph f xs z <-> MuRecsSpec n m f xs z.
+Proof.
+  pose proof (LEFT := @MuRecsGraph_complete). pose proof (RIGHT := @MuRecsGraph_sound). now firstorder.
+Qed.
+
+Fixpoint MuRec_isPartialFunction_aux (n : Arity) (f : MuRec n) (xs : Vector.t Value n) (z : Value) (SPEC : MuRecSpec n f xs z) {struct SPEC}
+  : forall z', MuRecGraph f xs z' -> z = z'
+with MuRecs_isPartialFunction_aux (n : Arity) (m : Arity) (fs : MuRecs n m) (xs : Vector.t Value n) (z : Vector.t Value m) (SPEC : MuRecsSpec n m fs xs z) {struct SPEC}
+  : forall z', MuRecsGraph fs xs z' -> z = z'.
+Proof.
+  - destruct SPEC; intros z' CALL.
+    + exact CALL.
+    + exact CALL.
+    + exact CALL.
+    + simpl in CALL. eapply MuRec_isPartialFunction_aux.
+      * exact SPEC.
+      * destruct CALL as (ys'&CALLs&CALL).
+        assert (claim : ys = ys').
+        { eapply MuRecs_isPartialFunction_aux; [exact g_spec | exact CALLs]. }
+        subst ys'. exact CALL.
+    + simpl in CALL. unfold V.tail in CALL; simpl in CALL. eapply MuRec_isPartialFunction_aux.
+      * eapply SPEC.
+      * exact CALL.
+    + simpl in CALL. destruct CALL as (y&ACC&CALL). unfold V.tail in ACC, CALL; simpl in ACC, CALL.
+      assert (claim : acc = y).
+      { eapply MuRec_isPartialFunction_aux.
+        - exact SPEC1.
+        - exact ACC. 
+      }
+      subst y. eapply MuRec_isPartialFunction_aux.
+      * exact SPEC2.
+      * exact CALL.
+    + simpl in CALL. destruct CALL as [MIN' CALL].
+      assert (NOT_LT : ~ z < z').
+      { intros LT. pose proof (MIN' z LT) as (p&p_gt_0&CALL').
+        enough (WTS : 0 = p) by lia.
+        eapply MuRec_isPartialFunction_aux.
+        - exact SPEC.
+        - exact CALL'.
+      }
+      assert (NOT_LT' : ~ z' < z).
+      { intros LT. pose proof (MIN z' LT) as (p&p_gt_0&CALL').
+        enough (WTS : p = 0) by lia.
+        eapply MuRec_isPartialFunction_aux. 
+        - exact CALL'.
+        - exact CALL.
+      }
+      lia.
+  - destruct SPEC; intros z' CALL'.
+    + revert z' CALL'. introVNil. i. reflexivity.
+    + revert z' CALL'. introVCons y' ys'. i. simpl in CALL'.
+      destruct CALL' as (y''&ys''&CALL''&CALLs''&EQ). rewrite <- EQ. eapply f_equal2.
+      * eapply MuRec_isPartialFunction_aux; [exact f_spec | exact CALL''].
+      * eapply MuRecs_isPartialFunction_aux; [exact SPEC | exact CALLs''].
+Qed.
+
+Theorem MuRec_isPartialFunction (n : Arity) (f : MuRec n) (xs : Vector.t Value n) (z : Value) (z' : Value)
+  (SPEC : MuRecSpec n f xs z)
+  (SPEC' : MuRecSpec n f xs z')
+  : z = z'.
+Proof.
+  eapply MuRec_isPartialFunction_aux; [exact SPEC | rewrite MuRecGraph_correct; exact SPEC'].
+Qed.
+
+Theorem MuRecs_isPartialFunction (n : Arity) (m : Arity) (fs : MuRecs n m) (xs : Vector.t Value n) (z : Vector.t Value m) (z' : Vector.t Value m)
+  (SPEC : MuRecsSpec n m fs xs z)
+  (SPEC' : MuRecsSpec n m fs xs z')
+  : z = z'.
+Proof.
+  eapply MuRecs_isPartialFunction_aux; [exact SPEC | rewrite MuRecsGraph_correct; exact SPEC'].
+Qed.
+
+Fixpoint MuRecInterpreter (n : Arity) (f : MuRec n) {struct f}
+  : forall xs, (exists z, MuRecSpec n f xs z) -> { z : Value | MuRecSpec n f xs z }
+with MuRecsInterpreter (n : Arity) (m : Arity) (fs : MuRecs n m) {struct fs}
+  : forall xs, (exists z, MuRecsSpec n m fs xs z) -> { z : Vector.t Value m | MuRecsSpec n m fs xs z }.
+Proof.
+  - destruct f; simpl; intros xs EXISTENCE.
+    + clear EXISTENCE. revert xs. introVCons x xs. revert xs. introVNil. exists (S x). econs 1.
+    + clear EXISTENCE. revert xs. introVNil. exists O. econs 2.
+    + clear EXISTENCE. exists (xs !! i). econs 3.
+    + assert (claim1 : exists z : Vector.t Value m, MuRecsSpec n m g xs z).
+      { destruct EXISTENCE as [z SPEC]. rewrite <- MuRecGraph_correct in SPEC. simpl in SPEC.
+        destruct SPEC as (ys&CALLs&CALL). exists ys. rewrite <- MuRecsGraph_correct. exact CALLs.
+      }
+      pose proof (MuRecsInterpreter n m g xs claim1) as [ys ys_spec].
+      assert (claim2 : exists z : Value, MuRecSpec m f ys z).
+      { destruct EXISTENCE as [z SPEC]. rewrite <- MuRecGraph_correct in SPEC. simpl in SPEC.
+        destruct SPEC as (ys'&CALLs&CALL). exists z. rewrite <- MuRecGraph_correct. replace ys with ys'. exact CALL.
+        eapply MuRecs_isPartialFunction.
+        - rewrite <- MuRecsGraph_correct. exact CALLs.
+        - exact ys_spec.
+      }
+      pose proof (MuRecInterpreter m f ys claim2) as [z z_spec]. exists z.
+      rewrite <- MuRecGraph_correct. simpl. exists ys. split.
+      * rewrite MuRecsGraph_correct. exact ys_spec.
+      * rewrite MuRecGraph_correct. exact z_spec.
+    + revert xs EXISTENCE. introVCons a xs. revert xs. induction a as [ | a IH]; simpl; i.
+      * assert (claim1 : exists z : Value, MuRecSpec n f1 xs z).
+        { destruct EXISTENCE as [z SPEC]. rewrite <- MuRecGraph_correct in SPEC. simpl in SPEC.
+          unfold V.tail in SPEC. simpl in SPEC. exists z. rewrite <- MuRecGraph_correct. exact SPEC.
+        }
+        pose proof (MuRecInterpreter n f1 xs claim1) as [z z_spec]. exists z.
+        rewrite <- MuRecGraph_correct. simpl. unfold V.tail. simpl. rewrite MuRecGraph_correct. exact z_spec.
+      * assert (claim1 : exists z : Value, MuRecSpec (S n) (MR_primRec f1 f2) (VCons n a xs) z).
+        { destruct EXISTENCE as [z SPEC]. rewrite <- MuRecGraph_correct in SPEC. simpl in SPEC.
+          unfold V.tail, V.head in SPEC. simpl in SPEC. destruct SPEC as [acc [CALL CALL']]. exists acc. rewrite <- MuRecGraph_correct. simpl.
+          unfold V.tail, V.head. simpl. exact CALL.
+        }
+        pose proof (IH xs claim1) as [acc acc_spec].
+        assert (claim2 : exists z : Value, MuRecSpec (S (S n)) f2 (VCons (S n) a (VCons n acc xs)) z).
+        { destruct EXISTENCE as [z SPEC]. rewrite <- MuRecGraph_correct in SPEC. simpl in SPEC.
+          unfold V.tail, V.head in SPEC. simpl in SPEC. destruct SPEC as [acc' [CALL CALL']].
+          assert (EQ : acc = acc').
+          { eapply MuRec_isPartialFunction.
+            - exact acc_spec.
+            - rewrite <- MuRecGraph_correct. simpl. unfold V.head, V.tail. simpl. exact CALL.
+          }
+          subst acc'. exists z. rewrite <- MuRecGraph_correct. exact CALL'.
+        }
+        pose proof (MuRecInterpreter (S (S n)) f2 (a :: acc :: xs) claim2) as [z z_spec].
+        exists z. econs 6. exact acc_spec. exact z_spec.
+    + pose (COUNTABLE := {| encode := id; decode := @Some nat; decode_encode (x : nat) := eq_refl |}). set (P := MuRecSpec n (MR_mu f) xs).
+      pose proof (@Acc_flip_search_step_P_0 nat COUNTABLE P EXISTENCE) as ACC.
+      assert (SEARCH : exists z, MuRecSpec n (MR_mu f) xs z /\ (forall x, x < z -> search_step P x (S x))).
+      { destruct EXISTENCE as [z z_spec]. exists z. split. exact z_spec.
+        rewrite <- MuRecGraph_correct in z_spec. simpl in z_spec.
+        destruct z_spec as [MIN z_spec]. intros y y_lt_z. pose proof (MIN y y_lt_z) as (p&p_gt_0&CALL).
+        eapply search_step_Some with (x := y). 2: reflexivity. unfold P. rewrite <- MuRecGraph_correct.
+        intros [MIN' y_spec]. enough (FALSE : p = 0) by lia. eapply MuRec_isPartialFunction.
+        - rewrite <- MuRecGraph_correct. exact CALL.
+        - rewrite <- MuRecGraph_correct. exact y_spec.
+      }
+      clear EXISTENCE. unfold P. set (F := fun x : nat => fun y : nat => MuRecSpec (S n) f (x :: xs) y).
+      assert (claim1 : forall x y1 y2 : nat, F x y1 -> F x y2 -> y1 = y2).
+      { intros x y1 y2. unfold F. intros SPEC1 SPEC2. eapply MuRec_isPartialFunction. eapply SPEC1. eapply SPEC2. }
+      assert (claim2 : forall x : nat, (exists y : nat, F x y) -> {y : nat | F x y}).
+      { unfold F. intros x EXISTENCE. exact (MuRecInterpreter (S n) f (x :: xs) EXISTENCE). }
+      assert (claim3 : exists x : nat, umin' F x).
+      { destruct SEARCH as [z [SEARCH STEP]]. exists z. red. unfold F. rewrite <- MuRecGraph_correct in SEARCH. simpl in SEARCH.
+        destruct SEARCH as [SEARCH MIN]. split.
+        - rewrite <- MuRecGraph_correct. exact MIN.
+        - intros i LT. pose proof (SEARCH i LT) as (p&p_gt_0&CALL). destruct p as [ | p'].
+          + lia.
+          + exists p'. rewrite <- MuRecGraph_correct. exact CALL.
+      }
+      pose proof (compute_umin' F claim1 claim2 claim3) as [x H_x].
+      exists x. rewrite <- MuRecGraph_correct. simpl. red in H_x. unfold F in H_x. destruct H_x as [SPEC MIN]. split.
+      * i. pose proof (MIN y H) as [p SPEC']. exists (S p). split. lia. rewrite <- MuRecGraph_correct in SPEC'. exact SPEC'.
+      * rewrite <- MuRecGraph_correct in SPEC. exact SPEC.
+  - destruct fs; intros xs EXISTENCE.
+    + exists []. econs 1.
+    + assert (claim1 : exists z : Value, MuRecSpec n f xs z).
+      { destruct EXISTENCE as [z SPEC]. rewrite <- MuRecsGraph_correct in SPEC. simpl in SPEC.
+        destruct SPEC as (y&ys&CALL&CALLs&EQ). exists y. rewrite <- MuRecGraph_correct. exact CALL.
+      }
+      assert (claim2 : exists z : Vector.t Value m, MuRecsSpec n m fs xs z).
+      { destruct EXISTENCE as [z SPEC]. rewrite <- MuRecsGraph_correct in SPEC. simpl in SPEC.
+        destruct SPEC as (y&ys&CALL&CALLs&EQ). exists ys. rewrite <- MuRecsGraph_correct. exact CALLs.
+      }
+      pose proof (MuRecInterpreter n f xs claim1) as [y y_spec].
+      pose proof (MuRecsInterpreter n m fs xs claim2) as [ys ys_spec].
+      exists (y :: ys). econs 2; [exact y_spec | exact ys_spec].
+Qed.
+
+End MU_RECURSIVE.
