theories/Logic/PrimRec.v
@@ -1,0 +1,381 @@
+Require Import PnV.Prelude.Prelude.
+Require Import PnV.Prelude.ConstructiveFacts.
+Require Import PnV.Data.Vector.
+
+Section PRIMITIVE_RECURSION. (* Reference: "https://github.com/princeton-vl/CoqGym/blob/master/coq_projects/goedel/primRec.v" *)
+
+#[local] Open Scope program_scope.
+
+Let arity : Set := nat.
+
+Fixpoint naryFun (n : arity) :=
+  match n with
+  | O => nat
+  | S n' => nat -> naryFun n'
+  end.
+
+Fixpoint naryRel (n : arity) :=
+  match n with
+  | O => Prop
+  | S n' => nat -> naryRel n'
+  end.
+
+Fixpoint eval_vec {n : arity} (xs : Vector.t nat n) : naryFun n -> nat :=
+  match xs with
+  | VNil => id
+  | VCons n' x xs' => fun f => eval_vec xs' (f x)
+  end.
+
+Fixpoint eval_const {n : arity} (m : nat) : naryFun n :=
+  match n with
+  | O => m
+  | S n' => const (eval_const m)
+  end.
+
+Fixpoint eval_proj {n : arity} (i : Fin.t n) : naryFun n :=
+  match i with
+  | FZ => eval_const
+  | FS i' => const (eval_proj i')
+  end.
+
+Lemma eval_proj_spec (n : arity) (i : Fin.t n) (xs : Vector.t nat n)
+  : eval_vec xs (eval_proj i) = xs !! i.
+Proof.
+  revert i. induction xs as [ | n x xs IH]; simpl.
+  - Fin.case0.
+  - Fin.caseS i.
+    + simpl. clear IH. revert x xs. induction n as [ | n IH]; simpl.
+      * intros x. introVNil. reflexivity.
+      * intros x. introVCons x' xs'. simpl. unfold const. eapply IH.
+    + eapply IH.
+Qed.
+
+Fixpoint eval_vec_1 {n : arity} {m : arity} (x : nat) (xs : Vector.t (naryFun (S n)) m) : Vector.t (naryFun n) m :=
+  match xs with
+  | VNil => VNil
+  | VCons m' f xs' => VCons m' (f x) (eval_vec_1 x xs')
+  end.
+
+Fixpoint eval_compose {n : arity} {m : arity} : Vector.t (naryFun n) m -> naryFun m -> naryFun n :=
+  match n with
+  | O => fun xs => eval_vec xs
+  | S n' => fun xs => fun f => fun x => eval_compose (eval_vec_1 x xs) f
+  end.
+
+Lemma eval_compose_spec (n : arity) (m : arity) (gs : Vector.t (naryFun n) m) (h : naryFun m) (xs : Vector.t nat n) (ys : Vector.t nat m) (z : nat)
+  (gs_spec : V.map (eval_vec xs) gs = ys)
+  (h_spec : eval_vec ys h = z)
+  : eval_vec xs (eval_compose gs h) = z.
+Proof.
+  revert m gs h xs ys z gs_spec h_spec. induction n as [ | n IH]; simpl.
+  - intros m gs h. introVNil. simpl. i.
+    assert (claim1 : ys = gs).
+    { rewrite <- gs_spec. clear ys z h gs_spec h_spec. induction gs as [ | n g gs IH]; simpl; trivial; f_equal; eauto. }
+    subst gs. clear gs_spec. exact h_spec.
+  - intros m gs h. introVCons x xs. simpl. i.
+    assert (claim2 : V.map (eval_vec xs) (eval_vec_1 x gs) = ys).
+    { rewrite <- gs_spec. clear ys gs_spec h_spec. clear z h IH. revert x xs. induction gs as [ | m g gs IH]; simpl.
+      - reflexivity.
+      - intros x xs. f_equal. eapply IH.
+    }
+    pose proof (claim3 := IH m (eval_vec_1 x gs) h xs ys z claim2 h_spec). congruence.
+Qed.
+
+Fixpoint eval_compose_2 {n : arity} : naryFun n -> naryFun (S n) -> naryFun n :=
+  match n with
+  | O => fun x => fun f => f x
+  | S n' => fun f => fun g => fun a => eval_compose_2 (f a) (fun x => g x a)
+  end.
+
+Lemma eval_compose_2_spec (n : arity) (g : naryFun n) (h : naryFun (S n)) (xs : Vector.t nat n) (a : nat) (z : nat)
+  (g_spec : eval_vec xs g = a)
+  (h_spec : eval_vec (a :: xs) h = z)
+  : eval_vec xs (eval_compose_2 g h) = z.
+Proof.
+  revert g h xs a z g_spec h_spec. induction n as [ | n IH]; simpl.
+  - intros g h. introVNil. simpl. i. cbv in *. congruence.
+  - intros g h. introVCons x xs. simpl. i.
+    exact (IH (g x) (fun a => h a x) xs a z g_spec h_spec).
+Qed.
+
+Fixpoint eval_primRec {n : arity} (g : naryFun n) (h : naryFun (S (S n))) (a : nat) : naryFun n :=
+  match a with
+  | O => g
+  | S a' => eval_compose_2 (eval_primRec g h a') (h a')
+  end.
+
+Inductive PrimRec : arity -> Set :=
+  | PR_succ : PrimRec 1
+  | PR_zero : PrimRec 0
+  | PR_proj (n : arity) (i : Fin.t n) : PrimRec n
+  | PR_compose (n : arity) (m : arity) (g : PrimRecs n m) (h : PrimRec m) : PrimRec n
+  | PR_primRec (n : arity) (g : PrimRec n) (h : PrimRec (S (S n))) : PrimRec (S n)
+with PrimRecs : arity -> arity -> Set :=
+  | PRs_nil (n : arity) : PrimRecs n 0
+  | PRs_cons (n : arity) (m : arity) (f : PrimRec n) (fs : PrimRecs n m) : PrimRecs n (S m).
+
+Section PrimRecs_case.
+
+Let cast (x : nat) (n : nat) (m : nat) (EQ : n = m) : PrimRecs x n -> PrimRecs x m :=
+  match EQ with
+  | eq_refl => fun xs => xs
+  end.
+
+Lemma PrimRecs_case0 (phi : forall x, PrimRecs x O -> Type)
+  (phi_nil : forall n, phi n (PRs_nil n))
+  : forall x, forall fs, phi x fs.
+Proof.
+  refine (fun x : nat =>
+    let claim1 (fs : PrimRecs x O) : forall H_eq : O = O, phi x (cast x O O H_eq fs) :=
+      match fs in PrimRecs x m return forall H_eq : m = O, phi x (cast x m O H_eq fs) with
+      | PRs_nil x => fun H_eq : O = O => _
+      | PRs_cons x n f' fs' => fun H_eq : S n = O => _
+      end
+    in _
+  ).
+  { intros fs. exact (claim1 fs eq_refl). }
+Unshelve.
+  - rewrite eq_pirrel_fromEqDec with (EQ1 := H_eq) (EQ2 := eq_refl).
+    exact (phi_nil x).
+  - inversion H_eq.
+Qed.
+
+Lemma PrimRecs_caseS {n' : nat} (phi : forall x, PrimRecs x (S n') -> Type)
+  (phi_cons: forall n, forall f', forall fs', phi n (PRs_cons n n' f' fs'))
+  : forall x, forall fs, phi x fs.
+Proof.
+  refine (fun x : nat =>
+    let claim1 (fs : PrimRecs x (S n')) : forall H_eq : S n' = S n', phi x (cast x (S n') (S n') H_eq fs) :=
+      match fs in PrimRecs x m return forall H_eq : m = S n', phi x (cast x m (S n') H_eq fs) with
+      | PRs_nil x => fun H_eq: O = S n' => _
+      | PRs_cons x n x' xs' => fun H_eq: S n = S n' => _
+      end
+    in _
+  ).
+  { intros fs. exact (claim1 fs eq_refl). }
+Unshelve.
+  - inversion H_eq.
+  - pose proof (f_equal Nat.pred H_eq) as n_eq_n'. simpl in n_eq_n'. subst n'.
+    rewrite eq_pirrel_fromEqDec with (EQ1 := H_eq) (EQ2 := eq_refl).
+    exact (phi_cons x x' xs').
+Qed.
+
+End PrimRecs_case.
+
+Fixpoint runPrimRec {n : arity} (f : PrimRec n) {struct f} : naryFun n :=
+  match f with
+  | PR_succ => S
+  | PR_zero => O
+  | PR_proj n i => eval_proj (n := n) i
+  | PR_compose n m g h => eval_compose (n := n) (m := m) (runPrimRecs g) (runPrimRec h)
+  | PR_primRec n g h => eval_primRec (n := n) (runPrimRec g) (runPrimRec h)
+  end
+with runPrimRecs {n : arity} {m : arity} (fs : PrimRecs n m) {struct fs} : Vector.t (naryFun n) m :=
+  match fs with
+  | PRs_nil n' => VNil
+  | PRs_cons n' m' f fs' => VCons m' (runPrimRec f) (runPrimRecs fs')
+  end.
+
+Lemma runPrimRec_unfold (n : arity) (f : PrimRec n) :
+  runPrimRec f =
+  match f with
+  | PR_succ => S
+  | PR_zero => O
+  | PR_proj n i => eval_proj i
+  | PR_compose n m g h => eval_compose (runPrimRecs g) (runPrimRec h)
+  | PR_primRec n g h => eval_primRec (runPrimRec g) (runPrimRec h)
+  end.
+Proof.
+  destruct f; reflexivity.
+Defined.
+
+Lemma runPrimRecs_unfold (n : arity) (m : arity) (fs : PrimRecs n m) :
+  runPrimRecs fs =
+  match fs with
+  | PRs_nil n' => VNil
+  | PRs_cons n' m' f fs' => VCons m' (runPrimRec f) (runPrimRecs fs')
+  end.
+Proof.
+  destruct fs; reflexivity.
+Defined.
+
+#[local] Close Scope list_scope.
+#[local] Open Scope vector_scope.
+
+#[local] Notation " [ ] " := (VNil).
+#[local] Notation " x :: xs " := (VCons _ x xs).
+#[local] Notation " [ x ] " := (VCons _ x VNil).
+
+Inductive PrimRecSpec : forall n : arity, PrimRec n -> Vector.t nat n -> nat -> Prop :=
+  | PR_succ_spec x
+    : PrimRecSpec 1 (PR_succ) [x] (S x)
+  | PR_zero_spec
+    : PrimRecSpec 0 (PR_zero) [] (O)
+  | PR_proj_spec n xs i
+    : PrimRecSpec n (PR_proj n i) xs (xs !! i)
+  | PR_compose_spec n m g h xs ys z
+    (g_spec : PrimRecsSpec n m g xs ys)
+    (h_spec : PrimRecSpec m h ys z)
+    : PrimRecSpec n (PR_compose n m g h) xs z
+  | PR_primRec_spec_O n g h xs z
+    (g_spec : PrimRecSpec n g xs z)
+    : PrimRecSpec (S n) (PR_primRec n g h) (O :: xs) z
+  | PR_primRec_spec_S n g h xs z a acc
+    (ACC : PrimRecSpec (S n) (PR_primRec n g h) (a :: xs) acc)
+    (h_spec : PrimRecSpec (S (S n)) h (a :: acc :: xs) z)
+    : PrimRecSpec (S n) (PR_primRec n g h) (S a :: xs) z
+with PrimRecsSpec : forall n : arity, forall m : arity, PrimRecs n m -> Vector.t nat n -> Vector.t nat m -> Prop :=
+  | PRs_nil_spec n xs
+    : PrimRecsSpec n (O) (PRs_nil n) xs []
+  | PRs_cons_spec n m xs y ys f fs
+    (f_spec : PrimRecSpec n f xs y)
+    (fs_spec : PrimRecsSpec n m fs xs ys)
+    : PrimRecsSpec n (S m) (PRs_cons n m f fs) xs (y :: ys).
+
+Fixpoint PrimRecGraph {n : arity} (f : PrimRec n) : Vector.t nat n -> nat -> Prop :=
+  match f with
+  | PR_succ => fun xs => fun z => S (V.head xs) = z
+  | PR_zero => fun xs => fun z => O = z
+  | PR_proj n i => fun xs => fun z => xs !! i = z
+  | PR_compose n m g h => fun xs => fun z => exists ys, PrimRecsGraph g xs ys /\ PrimRecGraph h ys z
+  | PR_primRec n g h => fun xs => nat_rect _ (fun z => PrimRecGraph g (V.tail xs) z) (fun a => fun ACC => fun z => exists y, ACC y /\ PrimRecGraph h (a :: y :: V.tail xs) z) (V.head xs)
+  end
+with PrimRecsGraph {n : arity} {m : arity} (fs : PrimRecs n m) : Vector.t nat n -> Vector.t nat m -> Prop :=
+  match fs with
+  | PRs_nil n => fun xs => fun z => [] = z
+  | PRs_cons n m f fs => fun xs => fun z => exists y, exists ys, PrimRecGraph f xs y /\ PrimRecsGraph fs xs ys /\ y :: ys = z
+  end.
+
+Fixpoint PrimRecGraph_sound (n : arity) (f : PrimRec n) {struct f}
+  : forall xs, forall z, PrimRecGraph f xs z -> PrimRecSpec n f xs z
+with PrimRecsGraph_sound (n : arity) (m : arity) (fs : PrimRecs n m) {struct fs}
+  : forall xs, forall z, PrimRecsGraph fs xs z -> PrimRecsSpec n m fs xs z.
+Proof.
+  - destruct f; intros xs z CALL.
+    + r in CALL. subst z. revert xs. introVCons x xs. revert xs. introVNil. cbv. econs 1.
+    + r in CALL. subst z. revert xs. introVNil. econs 2.
+    + r in CALL. subst z. econs 3.
+    + simpl in CALL. destruct CALL as (ys&CALLs&CALL). econs 4.
+      * eapply PrimRecsGraph_sound. exact CALLs.
+      * eapply PrimRecGraph_sound. exact CALL.
+    + simpl in CALL. revert xs CALL. introVCons a xs. revert z xs. induction a as [ | a ACC]; i.
+      * simpl in CALL. unfold V.tail in CALL. simpl in CALL. econs 5.
+        eapply PrimRecGraph_sound. exact CALL.
+      * simpl in CALL. destruct CALL as [y [CALL IH]]. unfold V.tail in CALL. simpl in CALL. unfold V.tail in IH. simpl in IH. econs 6.
+        { eapply ACC with (z := y). exact CALL. }
+        { eapply PrimRecGraph_sound. exact IH. }
+  - destruct fs; intros xs z CALL.
+    + simpl in CALL. subst z. econs 1.
+    + simpl in CALL. destruct CALL as [y [ys [CALL [CALLs ?]]]]. subst z. econs 2.
+      * eapply PrimRecGraph_sound. exact CALL.
+      * eapply PrimRecsGraph_sound. exact CALLs.
+Qed.
+
+Fixpoint PrimRecGraph_complete (n : arity) (f : PrimRec n) (xs : Vector.t nat n) (z : nat) (SPEC : PrimRecSpec n f xs z) {struct SPEC}
+  : PrimRecGraph f xs z
+with PrimRecsGraph_complete (n : arity) (m : arity) (fs : PrimRecs n m) (xs : Vector.t nat n) (z : Vector.t nat m) (SPEC : PrimRecsSpec n m fs xs z) {struct SPEC}
+  : PrimRecsGraph fs xs z.
+Proof.
+  - destruct SPEC; simpl.
+    + reflexivity.
+    + reflexivity.
+    + reflexivity.
+    + exists ys. split.
+      * eapply PrimRecsGraph_complete. exact g_spec.
+      * eapply PrimRecGraph_complete. exact SPEC.
+    + eapply PrimRecGraph_complete. exact SPEC.
+    + exists acc. unfold V.tail. simpl. split.
+      * apply PrimRecGraph_complete in SPEC1. exact SPEC1.
+      * apply PrimRecGraph_complete in SPEC2. exact SPEC2.
+  - destruct SPEC; simpl.
+    + reflexivity.
+    + exists y, ys. split. 
+      * eapply PrimRecGraph_complete. exact f_spec.
+      * split.
+        { eapply PrimRecsGraph_complete. exact SPEC. }
+        { reflexivity. }
+Qed.
+
+Theorem PrimRecGraph_correct (n : arity) (f : PrimRec n) (xs : Vector.t nat n) (z : nat)
+  : PrimRecGraph f xs z <-> PrimRecSpec n f xs z.
+Proof.
+  pose proof (LEFT := @PrimRecGraph_complete). pose proof (RIGHT := @PrimRecGraph_sound). now firstorder.
+Qed.
+
+Theorem PrimRecsGraph_correct (n : arity) (m : arity) (f : PrimRecs n m) (xs : Vector.t nat n) (z : Vector.t nat m)
+  : PrimRecsGraph f xs z <-> PrimRecsSpec n m f xs z.
+Proof.
+  pose proof (LEFT := @PrimRecsGraph_complete). pose proof (RIGHT := @PrimRecsGraph_sound). now firstorder.
+Qed.
+
+Fixpoint PrimRecSpec_sound (n : arity) (f : PrimRec n) (xs : Vector.t nat n) (z : nat) (SPEC : PrimRecSpec n f xs z) {struct SPEC}
+  : eval_vec xs (runPrimRec f) = z
+with PrimRecsSpec_sound (n : arity) (m : arity) (fs : PrimRecs n m) (xs : Vector.t nat n) (z : Vector.t nat m) (SPEC : PrimRecsSpec n m fs xs z) {struct SPEC}
+  : V.map (eval_vec xs) (runPrimRecs fs) = z.
+Proof.
+  - destruct SPEC.
+    + reflexivity.
+    + reflexivity.
+    + eapply eval_proj_spec.
+    + simpl. eapply eval_compose_spec.
+      * eapply PrimRecsSpec_sound. exact g_spec.
+      * eapply PrimRecSpec_sound. exact SPEC.
+    + simpl. eapply PrimRecSpec_sound. exact SPEC.
+    + simpl. eapply eval_compose_2_spec.
+      * apply PrimRecSpec_sound in SPEC1. simpl in SPEC1. exact SPEC1.
+      * apply PrimRecSpec_sound in SPEC2. simpl in SPEC2. simpl. exact SPEC2.
+  - destruct SPEC.
+    + reflexivity.
+    + simpl. eapply f_equal2.
+      * eapply PrimRecSpec_sound. exact f_spec.
+      * eapply PrimRecsSpec_sound. exact SPEC.
+Qed.
+
+Fixpoint PrimRecSpec_complete (n : arity) (f : PrimRec n) {struct f}
+  : forall xs, PrimRecSpec n f xs (eval_vec xs (runPrimRec f))
+with PrimRecsSpec_complete (n : arity) (m : arity) (fs : PrimRecs n m) {struct fs}
+  : forall xs, PrimRecsSpec n m fs xs (V.map (eval_vec xs) (runPrimRecs fs)).
+Proof.
+  - destruct f; simpl.
+    + introVCons x xs. revert xs. introVNil. simpl. econs 1.
+    + introVNil. econs 2.
+    + i. erewrite eval_proj_spec. econs 3.
+    + i. econs 4.
+      * eapply PrimRecsSpec_complete.
+      * erewrite eval_compose_spec.
+        { eapply PrimRecSpec_complete. }
+        { reflexivity. }
+        { reflexivity. }
+    + introVCons a xs. simpl. revert a xs. induction a as [ | a IH].
+      * simpl. i. econs 5. eapply PrimRecSpec_complete.
+      * simpl. i. econs 6. 
+        { eapply IH. }
+        { erewrite eval_compose_2_spec.
+          - eapply PrimRecSpec_complete.
+          - reflexivity.
+          - reflexivity.
+        }
+  - destruct fs; simpl.
+    + i. econs 1.
+    + i. econs 2.
+      * eapply PrimRecSpec_complete.
+      * eapply PrimRecsSpec_complete.
+Qed.
+
+Theorem PrimRecSpec_iff (n : arity) (f : PrimRec n) (xs : Vector.t nat n) (z : nat)
+  : PrimRecSpec n f xs z <-> eval_vec xs (runPrimRec f) = z.
+Proof.
+  split.
+  - intros SPEC. eapply PrimRecSpec_sound; exact SPEC.
+  - intros <-. eapply PrimRecSpec_complete.
+Qed.
+
+Theorem PrimRecsSpec_iff (n : arity) (m : arity) (f : PrimRecs n m) (xs : Vector.t nat n) (z : Vector.t nat m)
+  : PrimRecsSpec n m f xs z <-> V.map (eval_vec xs) (runPrimRecs f) = z.
+Proof.
+  split.
+  - intros SPEC. eapply PrimRecsSpec_sound; exact SPEC.
+  - intros <-. eapply PrimRecsSpec_complete.
+Qed.
+
+End PRIMITIVE_RECURSION.
