theories/Logic/PropositionalLogic.v
@@ -1,0 +1,539 @@
+Require Import PnV.Prelude.Prelude.
+
+#[local] Infix " \in " := E.In.
+#[local] Infix " \subseteq " := E.subset.
+#[local] Notation In := List.In.
+
+Definition propLetter : Set := nat.
+
+Inductive formula : Set :=
+  | AtomF (i : propLetter) : formula
+  | ContradictionF : formula
+  | NegationF (p1 : formula) : formula
+  | ConjunctionF (p1 : formula) (p2 : formula) : formula
+  | DisjunctionF (p1 : formula) (p2 : formula) : formula
+  | ImplicationF (p1 : formula) (p2 : formula) : formula
+  | BiconditionalF (p1 : formula) (p2 : formula) : formula.
+
+#[global]
+Instance propLetter_hasEqDec : hasEqDec propLetter :=
+  Nat.eq_dec.
+
+#[global]
+Instance formula_hasEqDec
+  : hasEqDec formula.
+Proof.
+  red. decide equality. eapply propLetter_hasEqDec.
+Defined.
+
+Fixpoint evalFormula (e : propLetter -> Prop) (p : formula) {struct p} : Prop :=
+  match p with
+  | AtomF i => e i
+  | ContradictionF => False
+  | NegationF p1 => ~ evalFormula e p1
+  | ConjunctionF p1 p2 => evalFormula e p1 /\ evalFormula e p2
+  | DisjunctionF p1 p2 => evalFormula e p1 \/ evalFormula e p2
+  | ImplicationF p1 p2 => evalFormula e p1 -> evalFormula e p2
+  | BiconditionalF p1 p2 => evalFormula e p1 <-> evalFormula e p2
+  end.
+
+Section PROPOSITONAL_LOGIC.
+
+Definition entails (Gamma : ensemble formula) (C : formula) : Prop :=
+  forall e : propLetter -> Prop, (forall H : formula, H \in Gamma -> evalFormula e H) -> evalFormula e C.
+
+Infix "⊨" := entails.
+
+#[local] Hint Unfold entails : core.
+
+Inductive infers (Gamma : ensemble formula) : forall C : formula, Prop :=
+  | ByAssumption C
+    (IN : C \in Gamma)
+    : Gamma ⊢ C
+  | ContradictionI A
+    (INFERS1 : Gamma ⊢ A)
+    (INFERS2 : Gamma ⊢ NegationF A)
+    : Gamma ⊢ ContradictionF
+  | ContradictionE A
+    (INFERS1 : Gamma ⊢ ContradictionF)
+    : Gamma ⊢ A
+  | NegationI A
+    (INFERS1 : E.insert A Gamma ⊢ ContradictionF)
+    : Gamma ⊢ NegationF A
+  | NegationE A
+    (INFERS1 : E.insert (NegationF A) Gamma ⊢ ContradictionF)
+    : Gamma ⊢ A
+  | ConjunctionI A B
+    (INFERS1 : Gamma ⊢ A)
+    (INFERS2 : Gamma ⊢ B)
+    : Gamma ⊢ ConjunctionF A B
+  | ConjunctionE1 A B
+    (INFERS1 : Gamma ⊢ ConjunctionF A B)
+    : Gamma ⊢ A
+  | ConjunctionE2 A B
+    (INFERS1 : Gamma ⊢ ConjunctionF A B)
+    : Gamma ⊢ B
+  | DisjunctionI1 A B
+    (INFERS1 : Gamma ⊢ A)
+    : Gamma ⊢ DisjunctionF A B
+  | DisjunctionI2 A B
+    (INFERS1 : Gamma ⊢ B)
+    : Gamma ⊢ DisjunctionF A B
+  | DisjunctionE A B C
+    (INFERS1 : Gamma ⊢ DisjunctionF A B)
+    (INFERS2 : E.insert A Gamma ⊢ C)
+    (INFERS3 : E.insert B Gamma ⊢ C)
+    : Gamma ⊢ C
+  | ImplicationI A B
+    (INFERS1 : E.insert A Gamma ⊢ B)
+    : Gamma ⊢ ImplicationF A B
+  | ImplicationE A B
+    (INFERS1 : Gamma ⊢ ImplicationF A B)
+    (INFERS2 : Gamma ⊢ A)
+    : Gamma ⊢ B
+  | BiconditionalI A B
+    (INFERS1 : E.insert A Gamma ⊢ B)
+    (INFERS2 : E.insert B Gamma ⊢ A)
+    : Gamma ⊢ BiconditionalF A B
+  | BiconditionalE1 A B
+    (INFERS1 : Gamma ⊢ BiconditionalF A B)
+    (INFERS2 : Gamma ⊢ A)
+    : Gamma ⊢ B
+  | BiconditionalE2 A B
+    (INFERS1 : Gamma ⊢ BiconditionalF A B)
+    (INFERS2 : Gamma ⊢ B)
+    : Gamma ⊢ A
+  where " Gamma ⊢ C " := (infers Gamma C) : type_scope.
+
+#[local] Hint Constructors infers : core.
+
+Lemma extend_entails Gamma Gamma' C
+  (ENTAILS: Gamma ⊨ C)
+  (SUBSET: Gamma \subseteq Gamma')
+  : Gamma' ⊨ C.
+Proof.
+  ii. eapply ENTAILS. eauto.
+Qed.
+
+Definition is_structure (Gamma : ensemble formula) : Prop :=
+  forall p : formula, p \in Gamma <-> evalFormula (E.preimage AtomF Gamma) p.
+
+Lemma structure_gives_its_subset_to_model (Gamma : ensemble formula) (Gamma' : ensemble formula)
+  (IS_STRUCTURE : is_structure Gamma')
+  (INCL : Gamma \subseteq Gamma')
+  : forall p, p \in Gamma -> evalFormula (E.preimage AtomF Gamma') p.
+Proof.
+  ii. eapply IS_STRUCTURE. eauto with *.
+Qed.
+
+Lemma Law_of_Excluded_Middle A
+  : E.empty ⊢ DisjunctionF A (NegationF A).
+Proof with repeat ((now left) || right).
+  eapply NegationE, ContradictionI.
+  - eapply DisjunctionI2, NegationI, ContradictionI.
+    + eapply DisjunctionI1, ByAssumption...
+    + eapply ByAssumption...
+  - eapply ByAssumption...
+Qed.
+
+Lemma Cut_property Gamma A B
+  (INFERS : Gamma ⊢ A)
+  (IMPLY : E.insert A Gamma ⊢ B)
+  : Gamma ⊢ B.
+Proof.
+  assert (claim : Gamma ⊢ ImplicationF A B).
+  { eapply ImplicationI; exact IMPLY. }
+  eapply ImplicationE; [exact claim | exact INFERS].
+Qed.
+
+#[local] Hint Resolve E.insert_monotonic : core.
+
+Lemma extend_infers Gamma Gamma' C
+  (INFERS : Gamma ⊢ C)
+  (SUBSET : Gamma \subseteq Gamma')
+  : Gamma' ⊢ C.
+Proof with eauto.
+  revert Gamma' SUBSET. induction INFERS; ii.
+  - eapply ByAssumption with (C := C)...
+  - eapply ContradictionI with (A := A)...
+  - eapply ContradictionE with (A := A)...
+  - eapply NegationI with (A := A)...
+  - eapply NegationE with (A := A)...
+  - eapply ConjunctionI with (A := A) (B := B)...
+  - eapply ConjunctionE1 with (A := A) (B := B)...
+  - eapply ConjunctionE2 with (A := A) (B := B)...
+  - eapply DisjunctionI1 with (A := A) (B := B)...
+  - eapply DisjunctionI2 with (A := A) (B := B)...
+  - eapply DisjunctionE with (A := A) (B := B) (C := C)...
+  - eapply ImplicationI with (A := A) (B := B)...
+  - eapply ImplicationE with (A := A) (B := B)...
+  - eapply BiconditionalI with (A := A) (B := B)...
+  - eapply BiconditionalE1 with (A := A) (B := B)...
+  - eapply BiconditionalE2 with (A := A) (B := B)...
+Qed.
+
+Lemma Deduction_thm (Gamma : ensemble formula) (H : formula) (C : formula)
+  : Gamma ⊢ ImplicationF H C <-> E.insert H Gamma ⊢ C.
+Proof.
+  split; intros INFERS.
+  - eapply ImplicationE with (A := H).
+    + enough (INFERS' : E.insert H Gamma ⊢ H).
+      { eapply extend_infers with (Gamma := Gamma); done!. }
+      eapply ByAssumption; done!.
+    + eapply ByAssumption; done!.
+  - eapply ImplicationI. exact INFERS.
+Qed.
+
+Section WEAK_COMPLETENESS.
+
+Definition ContradictionF_bool : bool :=
+  false.
+
+Definition NegationF_bool (b1 : bool) : bool :=
+  match b1 with
+  | true => false
+  | false => true
+  end.
+
+Definition ConjunctionF_bool (b1 : bool) (b2 : bool) : bool :=
+  match b1, b2 with
+  | true, true => true
+  | true, false => false
+  | false, true => false
+  | false, false => false
+  end.
+
+Definition DisjunctionF_bool (b1 : bool) (b2 : bool) : bool :=
+  match b1, b2 with
+  | true, true => true
+  | true, false => true
+  | false, true => true
+  | false, false => false
+  end.
+
+Definition ImplicationF_bool (b1 : bool) (b2 : bool) : bool :=
+  match b1, b2 with
+  | true, true => true
+  | true, false => false
+  | false, true => true
+  | false, false => true
+  end.
+
+Definition BiconditionalF_bool (b1 : bool) (b2 : bool) : bool :=
+  match b1, b2 with
+  | true, true => true
+  | true, false => false
+  | false, true => false
+  | false, false => true
+  end.
+
+Fixpoint eval_bool (env : propLetter -> bool) (p : formula) {struct p} : bool :=
+  match p with
+  | AtomF i => env i
+  | ContradictionF => ContradictionF_bool
+  | NegationF p1 => NegationF_bool (eval_bool env p1)
+  | ConjunctionF p1 p2 => ConjunctionF_bool (eval_bool env p1) (eval_bool env p2)
+  | DisjunctionF p1 p2 => DisjunctionF_bool (eval_bool env p1) (eval_bool env p2)
+  | ImplicationF p1 p2 => ImplicationF_bool (eval_bool env p1) (eval_bool env p2)
+  | BiconditionalF p1 p2 => BiconditionalF_bool (eval_bool env p1) (eval_bool env p2)
+  end.
+
+Lemma eval_bool_true_iff (e : propLetter -> bool) (p : formula)
+  : eval_bool e p = true <-> evalFormula (fun i => if e i then True else False) p.
+Proof.
+  revert e. induction p as [i | | p1 IH1 | p1 IH1 p2 IH2 | p1 IH1 p2 IH2 | p1 IH1 p2 IH2 | p1 IH1 p2 IH2]; simpl; ii.
+  - destruct (e i) as [ | ]; done!.
+  - done!.
+  - specialize IH1 with (e := e). destruct (eval_bool e p1) as [ | ]; done!.
+  - specialize IH1 with (e := e). specialize IH2 with (e := e). destruct (eval_bool e p1) as [ | ], (eval_bool e p2) as [ | ]; done!.
+  - specialize IH1 with (e := e). specialize IH2 with (e := e). destruct (eval_bool e p1) as [ | ], (eval_bool e p2) as [ | ]; done!.
+  - specialize IH1 with (e := e). specialize IH2 with (e := e). destruct (eval_bool e p1) as [ | ], (eval_bool e p2) as [ | ]; done!.
+  - specialize IH1 with (e := e). specialize IH2 with (e := e). destruct (eval_bool e p1) as [ | ], (eval_bool e p2) as [ | ]; done!.
+Qed.
+
+Theorem eval_bool_spec (e : propLetter -> bool) (p : formula)
+  (e' := fun i => if e i then True else False)
+  : forall b, eval_bool e p = b <-> (if b then evalFormula e' p else ~ evalFormula e' p).
+Proof.
+  intros [ | ].
+  - eapply eval_bool_true_iff with (e := e) (p := p).
+  - subst e'. rewrite <- eval_bool_true_iff with (e := e) (p := p).
+    destruct (eval_bool e p) as [ | ]; done.
+Qed.
+
+Definition finite_entails (Gamma : list formula) (C : formula) : Prop :=
+  forall e : propLetter -> bool, (forall H, In H Gamma -> eval_bool e H = true) -> eval_bool e C = true.
+
+#[local] Hint Unfold finite_entails : simplication_hints.
+
+Lemma finite_entails_monotonic (Gamma : list formula) (Gamma' : list formula) (C : formula)
+  (ENTAILS : finite_entails Gamma C)
+  (SUBSET : forall H, In H Gamma -> In H Gamma')
+  : finite_entails Gamma' C.
+Proof.
+  done!.
+Qed.
+
+Lemma finite_entails_premise (Gamma : list formula) (H : formula)
+  (IN : In H Gamma)
+  : finite_entails Gamma H.
+Proof.
+  eapply finite_entails_monotonic with (Gamma := [H]).
+  - ii. done!.
+  - now simpl; intros ? [-> | []].
+Qed.
+
+Theorem finite_entails_if_entails (Gamma : list formula) (C : formula)
+  (ENTAILS : E.fromList Gamma ⊨ C)
+  : finite_entails Gamma C.
+Proof.
+  red in ENTAILS. intros e Gamma_SAT. rewrite -> eval_bool_spec with (e := e).
+  eapply ENTAILS. ii. rewrite <- eval_bool_spec with (e := e) (b := true).
+  eapply Gamma_SAT. done!.
+Qed.
+
+Fixpoint occurs (i : propLetter) (p : formula) {struct p} : Prop :=
+  match p with
+  | AtomF i' => i = i'
+  | ContradictionF => False
+  | NegationF p1 => occurs i p1
+  | ConjunctionF p1 p2 => occurs i p1 \/ occurs i p2
+  | DisjunctionF p1 p2 => occurs i p1 \/ occurs i p2
+  | ImplicationF p1 p2 => occurs i p1 \/ occurs i p2
+  | BiconditionalF p1 p2 => occurs i p1 \/ occurs i p2
+  end.
+
+Definition gen_context_for (env : propLetter -> bool) : list propLetter -> list formula :=
+  L.map (fun i : propLetter => if env i then AtomF i else NegationF (AtomF i)).
+
+Lemma infers_dec (C : formula)
+  : { ls : list propLetter | ⟪ OCCURS : forall l, In l ls <-> occurs l C ⟫ /\ ⟪ INFERS_DEC : forall e, let Gamma := E.fromList (gen_context_for e ls) in if eval_bool e C then Gamma ⊢ C else Gamma ⊢ NegationF C ⟫ }.
+Proof.
+  unnw.  revert C.
+  assert (AUX1 : forall e, forall ls1, forall ls2, E.fromList (gen_context_for e ls1) \subseteq E.fromList (gen_context_for e (ls1 ++ ls2))).
+  { intros e ls1 lhs2 p IN. s!. unfold gen_context_for in *. rewrite L.in_map_iff in *. destruct IN as [l [<- IN]]. exists l. done!. }
+  assert (AUX2 : forall e, forall ls1, forall ls2, E.fromList (gen_context_for e ls2) \subseteq E.fromList (gen_context_for e (ls1 ++ ls2))).
+  { intros e ls1 lhs2 p IN. s!. unfold gen_context_for in *. rewrite L.in_map_iff in *. destruct IN as [l [<- IN]]. exists l. done!. }
+  intros p. induction p as [i | | p1 IH1 | p1 IH1 p2 IH2 | p1 IH1 p2 IH2 | p1 IH1 p2 IH2 | p1 IH1 p2 IH2].
+  - exists [i]. split; i.
+    + ss!.
+    + simpl. destruct (e i) as [ | ]; eapply ByAssumption; done!.
+  - exists []. split; i.
+    + ss!.
+    + simpl. eapply NegationI. eapply ContradictionI with (A := ContradictionF).
+      * eapply ByAssumption. done!.
+      * eapply ContradictionE. eapply ByAssumption. done!.
+  - destruct IH1 as (ls1 & IFF1 & INFERS1). exists ls1. split; i.
+    + ss!.
+    + simpl. specialize INFERS1 with (e := e). simpl in INFERS1.
+      destruct (eval_bool e p1) as [ | ] eqn: OBS1; cbn.
+      * eapply NegationI. eapply ContradictionI with (A := p1).
+        { eapply extend_infers with (Gamma := E.fromList (gen_context_for e ls1)); done!. }
+        { eapply ByAssumption. done!. }
+      * done!.
+  - destruct IH1 as (ls1 & IFF1 & INFERS1), IH2 as (ls2 & IFF2 & INFERS2). exists (ls1 ++ ls2). split; i.
+    + ss!.
+    + simpl. specialize INFERS1 with (e := e). specialize INFERS2 with (e := e). simpl in INFERS1, INFERS2.
+      destruct (eval_bool e p1) as [ | ] eqn: OBS1; destruct (eval_bool e p2) as [ | ] eqn: OBS2; cbn; trivial.
+      * eapply ConjunctionI.
+        { eapply extend_infers with (Gamma := E.fromList (gen_context_for e ls1)); trivial. }
+        { eapply extend_infers with (Gamma := E.fromList (gen_context_for e ls2)); trivial. }
+      * assert (claim1 : E.insert (ConjunctionF p1 p2) (E.fromList (gen_context_for e (ls1 ++ ls2))) ⊢ NegationF p2).
+        { eapply extend_infers with (Gamma := E.fromList (gen_context_for e (ls1 ++ ls2))); trivial.
+          - eapply extend_infers with (Gamma := E.fromList (gen_context_for e ls2)); trivial.
+          - done!.
+        }
+        eapply NegationI. eapply ContradictionI with (Gamma := E.insert (ConjunctionF p1 p2) (E.fromList (gen_context_for e (ls1 ++ ls2)))) (A := p2); trivial.
+        eapply ConjunctionE2 with (A := p1). eapply ByAssumption. done!.
+      * assert (claim1 : E.insert (ConjunctionF p1 p2) (E.fromList (gen_context_for e (ls1 ++ ls2))) ⊢ NegationF p1).
+        { eapply extend_infers with (Gamma := E.fromList (gen_context_for e (ls1 ++ ls2))); trivial.
+          - eapply extend_infers with (Gamma := E.fromList (gen_context_for e ls1)); trivial.
+          - done!.
+        }
+        eapply NegationI. eapply ContradictionI with (Gamma := E.insert (ConjunctionF p1 p2) (E.fromList (gen_context_for e (ls1 ++ ls2)))) (A := p1); trivial.
+        eapply ConjunctionE1 with (B := p2). eapply ByAssumption. done!.
+      * assert (claim1 : E.insert (ConjunctionF p1 p2) (E.fromList (gen_context_for e (ls1 ++ ls2))) ⊢ NegationF p1).
+        { eapply extend_infers with (Gamma := E.fromList (gen_context_for e ls1)); trivial. ii. right. eapply AUX1; done. }
+        assert (claim2 : E.insert (ConjunctionF p1 p2) (E.fromList (gen_context_for e (ls1 ++ ls2))) ⊢ NegationF p2).
+        { eapply extend_infers with (Gamma := E.fromList (gen_context_for e ls2)); trivial. ii. right. eapply AUX2; done. }
+        eapply NegationI. eapply ContradictionI with (Gamma := E.insert (ConjunctionF p1 p2) (E.fromList (gen_context_for e (ls1 ++ ls2)))) (A := p1); trivial.
+        eapply ConjunctionE1 with (B := p2). eapply ByAssumption. done!.
+  - destruct IH1 as (ls1 & IFF1 & INFERS1), IH2 as (ls2 & IFF2 & INFERS2). simpl in INFERS1, INFERS2. exists (ls1 ++ ls2). split; i.
+    + ss!.
+    + simpl. specialize INFERS1 with (e := e); specialize INFERS2 with (e := e).
+      destruct (eval_bool e p1) as [ | ] eqn: OBS1; destruct (eval_bool e p2) as [ | ] eqn: OBS2; cbn.
+      * eapply DisjunctionI1. eapply extend_infers with (Gamma := E.fromList (gen_context_for e ls1)); trivial.
+      * eapply DisjunctionI1. eapply extend_infers with (Gamma := E.fromList (gen_context_for e ls1)); trivial.
+      * eapply DisjunctionI2. eapply extend_infers with (Gamma := E.fromList (gen_context_for e ls2)); trivial.
+      * eapply NegationI. eapply DisjunctionE with (A := p1) (B := p2).
+        { eapply ByAssumption; done!. }
+        { eapply ContradictionI with (A := p1).
+          - eapply ByAssumption; done!.
+          - eapply extend_infers with (Gamma := E.fromList (gen_context_for e ls1)); trivial.
+            ii. right. right. eapply AUX1; done.
+        }
+        { eapply ContradictionI with (A := p2).
+          - eapply ByAssumption; done!.
+          - eapply extend_infers with (Gamma := E.fromList (gen_context_for e ls2)); trivial.
+            ii. right. right. eapply AUX2; done!.
+        }
+  - destruct IH1 as (ls1 & IFF1 & INFERS1), IH2 as (ls2 & IFF2 & INFERS2). exists (ls1 ++ ls2). split; i.
+    + ss!.
+    + simpl. specialize INFERS1 with (e := e). specialize INFERS2 with (e := e). simpl in INFERS1, INFERS2.
+      destruct (eval_bool e p1) as [ | ] eqn: OBS1; destruct (eval_bool e p2) as [ | ] eqn: OBS2; cbn; trivial.
+      * eapply ImplicationI. eapply extend_infers with (Gamma := E.fromList (gen_context_for e ls2)); trivial.
+        ii. right. eapply AUX2; done.
+      * eapply NegationI. eapply ContradictionI with (A := p2).
+        { eapply ImplicationE with (A := p1).
+          - eapply ByAssumption. done!.
+          - eapply extend_infers with (Gamma := E.fromList (gen_context_for e ls1)); trivial.
+            ii. right. eapply AUX1. done!.
+        }
+        { eapply NegationI. eapply ContradictionI with (A := p2).
+          - eapply ByAssumption. done!.
+          - eapply extend_infers with (Gamma := E.fromList (gen_context_for e ls2)); trivial.
+            ii. right. right. eapply AUX2; done!.
+        }
+      * eapply ImplicationI. eapply extend_infers with (Gamma := E.fromList (gen_context_for e ls2)).
+        { eapply INFERS2. }
+        { ii. right. eapply AUX2; done!. }
+      * eapply ImplicationI. eapply ContradictionE. eapply ImplicationE with (A := NegationF p1).
+        { eapply ImplicationI. eapply ContradictionI with (A := p1).
+          - eapply ByAssumption. done!.
+          - eapply ByAssumption. done!.
+        }
+        { eapply extend_infers with (Gamma := E.fromList (gen_context_for e ls1)); trivial.
+          ii. right. eapply AUX1. done!.
+        }
+  - destruct IH1 as (ls1 & IFF1 & INFERS1), IH2 as (ls2 & IFF2 & INFERS2). exists (ls1 ++ ls2). split; i.
+    + ss!.
+    + simpl. specialize INFERS1 with (e := e). specialize INFERS2 with (e := e). simpl in INFERS1, INFERS2.
+      destruct (eval_bool e p1) as [ | ] eqn: OBS1; destruct (eval_bool e p2) as [ | ] eqn: OBS2; cbn; trivial.
+      * eapply BiconditionalI.
+        { eapply extend_infers with (Gamma := E.fromList (gen_context_for e ls2)); trivial.
+          ii. right. eapply AUX2. done!.
+        }
+        { eapply extend_infers with (Gamma := E.fromList (gen_context_for e ls1)); trivial.
+          ii. right. eapply AUX1. done!.
+        }
+      * eapply NegationI.
+        { eapply ContradictionI with (A := p2).
+          - eapply BiconditionalE1 with (A := p1).
+            + eapply ByAssumption. done!.
+            + eapply extend_infers with (Gamma := E.fromList (gen_context_for e ls1)); trivial.
+              ii. right. eapply AUX1; done!.
+          - eapply extend_infers with (Gamma := E.fromList (gen_context_for e ls2)); trivial.
+            ii. right. eapply AUX2; done!.
+        }
+      * eapply NegationI.
+        { eapply ContradictionI with (A := p1).
+          - eapply BiconditionalE2 with (B := p2).
+            + eapply ByAssumption. done!.
+            + eapply extend_infers with (Gamma := E.fromList (gen_context_for e ls2)); trivial.
+              ii. right. eapply AUX2; done!.
+          - eapply extend_infers with (Gamma := E.fromList (gen_context_for e ls1)); trivial.
+            ii. right. eapply AUX1; done!.
+        }
+      * eapply BiconditionalI.
+        { eapply NegationE. eapply ContradictionI with (A := p1).
+          - eapply ByAssumption. done!.
+          - eapply extend_infers with (Gamma := E.fromList (gen_context_for e ls1)); trivial.
+            ii. right. right. eapply AUX1; done!.
+        }
+        { eapply NegationE. eapply ContradictionI with (A := p2).
+          - eapply ByAssumption. done!.
+          - eapply extend_infers with (Gamma := E.fromList (gen_context_for e ls2)); trivial.
+            ii. right. right. eapply AUX2; done!.
+        }
+Qed.
+
+Lemma is_theorem_if_is_deducible_for_any_gen_context (C : formula) (ls : list propLetter)
+  (OCCURS : forall i : propLetter, In i ls -> occurs i C)
+  (INFERS : forall e : propLetter -> bool, E.fromList (gen_context_for e ls) ⊢ C)
+  : E.fromList [] ⊢ C.
+Proof.
+  revert ls C OCCURS INFERS.
+  assert (MAP_EXT : forall ls : list propLetter, forall f1 : propLetter -> formula, forall f2 : propLetter -> formula,
+    forall EXT : forall l : propLetter, In l ls -> f1 l = f2 l,
+    List.map f1 ls = List.map f2 ls
+  ).
+  { induction ls as [ | l ls IH]; simpl; ii; [ | f_equal]; eauto with *. }
+  induction ls as [ | i ls IH]; simpl; i.
+  - eapply INFERS. exact (fun _ => false).
+  - destruct (List.in_dec Nat.eq_dec i ls) as [YES | NO].
+    + eapply IH. ss!. intros e. eapply extend_infers with (Gamma := E.fromList (gen_context_for e (i :: ls))).
+      * eapply INFERS.
+      * simpl. destruct (e i) as [ | ] eqn: H_OBS; intros H IN.
+        { s!. destruct IN as [<- | IN]; unfold gen_context_for in *; ss!. exists i. rewrite H_OBS; ss!. }
+        { s!. destruct IN as [<- | IN]; unfold gen_context_for in *; ss!. exists i. rewrite H_OBS; ss!. }
+    + eapply IH. done!. intros e. destruct (e i) as [ | ] eqn: H_OBS.
+      * set (e' := fun l : propLetter => if eq_dec i l then false else e l).
+        assert (INFERS' : E.insert (NegationF (AtomF i)) (E.fromList (gen_context_for e' ls)) ⊢ C).
+        { specialize INFERS with (e := e'). unfold e' in INFERS. destruct (eq_dec i i) as [EQ | NE]; [clear EQ | contradiction].
+          fold e' in INFERS. eapply extend_infers with (Gamma := E.fromList (NegationF (AtomF i) :: gen_context_for e' ls)); ss!.
+        }
+        assert (H_EQ : gen_context_for e ls = gen_context_for e' ls).
+        { specialize MAP_EXT with (ls := ls) (f1 := fun i => if e i then AtomF i else NegationF (AtomF i)) (f2 := fun i => if e' i then AtomF i else NegationF (AtomF i)). 
+          unfold gen_context_for. eapply MAP_EXT. intros i' IN'. unfold e'. destruct (eq_dec i i') as [EQ | NE].
+          - subst i'. contradiction.
+          - reflexivity.
+        }
+        assert (claim1 : E.insert (NegationF (AtomF i)) (E.fromList (gen_context_for e ls)) ⊢ C).
+        { rewrite -> H_EQ; trivial. }
+        assert (claim2 : E.fromList (gen_context_for e ls) ⊢ DisjunctionF (AtomF i) (NegationF (AtomF i))).
+        { eapply extend_infers with (Gamma := E.empty); [eapply Law_of_Excluded_Middle | done]. }
+        eapply DisjunctionE with (A := AtomF i) (B := NegationF (AtomF i)) (C := C); trivial.
+        specialize INFERS with (e := e). rewrite H_OBS in INFERS.
+        eapply extend_infers with (Gamma := E.fromList (AtomF i :: gen_context_for e ls)); ss!.
+      * set (e' := fun l : propLetter => if eq_dec i l then true else e l).
+        assert (INFERS' : E.insert (AtomF i) (E.fromList (gen_context_for e' ls)) ⊢ C).
+        { specialize INFERS with (e := e'). unfold e' in INFERS. destruct (eq_dec i i) as [EQ | NE]; [clear EQ | contradiction].
+          fold e' in INFERS. eapply extend_infers with (Gamma := E.fromList (AtomF i :: gen_context_for e' ls)); ss!.
+        }
+        assert (H_EQ : gen_context_for e ls = gen_context_for e' ls).
+        { specialize MAP_EXT with (ls := ls) (f1 := fun i => if e i then AtomF i else NegationF (AtomF i)) (f2 := fun i => if e' i then AtomF i else NegationF (AtomF i)). 
+          unfold gen_context_for. eapply MAP_EXT. intros i' IN'. unfold e'. destruct (eq_dec i i') as [EQ | NE].
+          - subst i'. contradiction.
+          - reflexivity.
+        }
+        assert (claim1 : E.insert (AtomF i) (E.fromList (gen_context_for e ls)) ⊢ C).
+        { rewrite -> H_EQ; trivial. }
+        assert (claim2 : E.fromList (gen_context_for e ls) ⊢ DisjunctionF (AtomF i) (NegationF (AtomF i))).
+        { eapply extend_infers with (Gamma := E.empty); [eapply Law_of_Excluded_Middle | done]. }
+        eapply DisjunctionE with (A := AtomF i) (B := NegationF (AtomF i)) (C := C); trivial.
+        specialize INFERS with (e := e). rewrite H_OBS in INFERS.
+        eapply extend_infers with (Gamma := E.fromList (NegationF (AtomF i) :: gen_context_for e ls)); ss!.
+Qed.
+
+Theorem tautology_is_theorem (C : formula)
+  (ENTAILS : finite_entails [] C)
+  : E.fromList [] ⊢ C.
+Proof.
+  unfold finite_entails in ENTAILS. pose proof (infers_dec C) as (ls & ?); des.
+  eapply is_theorem_if_is_deducible_for_any_gen_context with (ls := ls).
+  - done!.
+  - intros e. specialize INFERS_DEC with (e := e). specialize ENTAILS with (e := e).
+    destruct (eval_bool e C) as [ | ] eqn: OBS; trivial. discriminate ENTAILS. done!.
+Qed.
+
+Corollary weak_completeness (Gamma : list formula) (C : formula)
+  (ENTAILS : finite_entails Gamma C)
+  : E.fromList Gamma ⊢ C.
+Proof.
+  revert C ENTAILS. induction Gamma as [ | H Gamma IH].
+  - exact tautology_is_theorem.
+  - ii. eapply extend_infers with (Gamma := E.insert H (E.fromList Gamma)).
+    { eapply ImplicationE with (A := H).
+      - eapply extend_infers with (Gamma := E.fromList Gamma).
+        + eapply IH. intros e Gamma_SAT. simpl. red in ENTAILS. destruct (eval_bool e H) as [ | ] eqn: H_OBS.
+          * rewrite ENTAILS with (e := e); trivial; simpl. intros A [<- | IN]; eauto.
+          * now destruct (eval_bool e C) as [ | ].
+        + done!.
+      - eapply ByAssumption. done!.
+    }
+    { now intros A [<- | IN]; [left | right]. }
+Qed.
+
+End WEAK_COMPLETENESS.
+
+End PROPOSITONAL_LOGIC.
